examples/lowparse/LowParse.Examples.Extract.fst
@@ -3,6 +3,6 @@ open LowParse
 open LowParse.Examples
 
 inline_for_extraction
-let validate_fstar_test
-: stateful_validator parse_fstar_test
-= validate_fstar_test
+let validate_test
+: stateful_validator parse_test
+= validate_test
