examples/lowparse/LowParse.Int.fst
@@ -45,21 +45,24 @@ let validate_u32_st = validate_total_constant_size 4ul parse_u32
 [@"substitute"]
 inline_for_extraction
 let parse_u8_st_nochk :
-    parser_st_nochk parse_u8 = fun input ->
-    let b0 = Buffer.index input.S.p 0ul in
-    (b0, 1ul)
+    parser_st_nochk parse_u8 =
+    parse_total_constant_size_nochk 1ul (fun (input: S.bslice) ->
+      Buffer.index input.S.p 0ul
+    )
 
 [@"substitute"]
 inline_for_extraction
-let parse_u8_st : parser_st parse_u8 =
-  parse_total_constant_size 1ul parse_u8_st_nochk
+let parse_u8_st :
+    parser_st parse_u8 =
+    parse_total_constant_size 1ul parse_u8_st_nochk
 
 [@"substitute"]
 inline_for_extraction
 let parse_u16_st_nochk :
-  parser_st_nochk parse_u16 = fun input ->
-  let n = C.load16_be (S.truncated_slice input 2ul).S.p in
-  (n, 2ul)
+  parser_st_nochk parse_u16 =
+  parse_total_constant_size_nochk 2ul (fun (input: S.bslice) ->
+    C.load16_be (S.truncated_slice input 2ul).S.p
+  )
 
 [@"substitute"]
 inline_for_extraction
@@ -69,9 +72,10 @@ let parse_u16_st : parser_st parse_u16 =
 [@"substitute"]
 inline_for_extraction
 let parse_u32_st_nochk :
-  parser_st_nochk (parse_u32) = fun input ->
-  let n = C.load32_be (S.truncated_slice input 4ul).S.p in
-  (n, 4ul)
+  parser_st_nochk (parse_u32) = 
+  parse_total_constant_size_nochk 4ul (fun input ->
+    C.load32_be (S.truncated_slice input 4ul).S.p
+  )
 
 [@"substitute"]
 inline_for_extraction
